added documentation, started coherence

.lake/build/ir/Games/gameLib/Basic.c
@@ -192,13 +192,10 @@ return x_3;
 LEAN_EXPORT lean_object* l_Turn__from__hist___rarg(lean_object* x_1) {
 _start:
 {
-lean_object* x_2; lean_object* x_3; lean_object* x_4; lean_object* x_5; 
+lean_object* x_2; lean_object* x_3; 
 x_2 = lean_unsigned_to_nat(0u);
 x_3 = l_List_lengthTRAux___rarg(x_1, x_2);
-x_4 = lean_unsigned_to_nat(1u);
-x_5 = lean_nat_add(x_3, x_4);
-lean_dec(x_3);
-return x_5;
+return x_3;
 }
 }
 LEAN_EXPORT lean_object* l_Turn__from__hist(lean_object* x_1) {
